#+TITLE: 779 K_th_symbol_in_grammar


#+begin_src c++
class Solution {
public:
    int kthGrammar(int n, int k) {
        // just simple bfs
        queue<int> bfs;
        bfs.push(0);

        for(int main = 1; main <= n; main++) {
            int len = bfs.size();

            for(int i = 0; i < len; i++) {
                int element = bfs.front();
                bfs.pop();

                if (main == n && i == (k - 1)) {
                    return element;
                }

                if (element == 0) {
                    bfs.push(0);
                    bfs.push(1);
                } else if(element == 1) {
                    bfs.push(1);
                    bfs.push(0);
                }
            }
        }

        return 0;
    }
};
#+end_src

The length of the nth row is double the length of the (n-1)th row.
If k is in the first half of the nth row, the symbol at position k in the nth row is the same as the symbol at position k in the (n-1)th row.
If k is in the second half of the nth row, the symbol at position k in the nth row is the opposite of the symbol at position (k - length of (n-1)th row) in the (n-1)th row.

#+begin_src c++
class Solution {
public:
    int kthGrammar(int n, int k) {
        if (n == 1) { return 0; }
        int length = 1 << (n - 2);

        if (k <= length) {
          return kthGrammar(n - 1, k);
        } else {
          return 1 - kthGrammar(n - 1, k - length);
        }
    }
};
#+end_src
